steel/Veritas.Steel.MainWorkerChannel.fsti
@@ -5,41 +5,35 @@ module G = FStar.Ghost
 open Steel.Effect
 
 module TSM = Veritas.ThreadStateModel
-module VTypes = Veritas.Formats.Types
+module Formats = Veritas.Formats.Types
 module Model = Veritas.Steel.VerifierModel
 module Awc = Veritas.Steel.ApplicationWorkerChannel
 
-
-val epoch_id : Type0
-
-val initial_thread_state_model (id:epoch_id)
-  : tsm:TSM.thread_state_model{tsm.TSM.model_failed == false}
-
-noeq
-type epoch_hash_entry (c:G.erased Awc.ch) = {
-  e_id : epoch_id;
-  entries : s:G.erased (Seq.seq VTypes.vlog_entry){exists n. Awc.sent_s c s n};
-  hadd : TSM.model_hash;
-  hevict : h:TSM.model_hash{
-    let tsm = Model.verify_model (initial_thread_state_model e_id) entries in
-    not tsm.TSM.model_failed      /\
-    tsm.TSM.model_hadd == hadd    /\
-    tsm.TSM.model_hevict == h};
-}
+// noeq
+// type epoch_hash_entry (c:G.erased Awc.ch) = {
+//   e_id : Formats.epoch_id;
+//   entries : s:G.erased (Seq.seq Formats.vlog_entry){exists n. Awc.sent_s c s n};
+//   hadd : TSM.model_hash;
+//   hevict : h:TSM.model_hash{
+//     let tsm = Model.verify_model (TSM.initial_thread_state_model e_id) entries in
+//     not tsm.TSM.model_failed      /\
+//     tsm.TSM.model_hadd == hadd    /\
+//     tsm.TSM.model_hevict == h};
+// }
 
 val ch : Type0
 
 val reader (c:ch) : vprop
 val writer (c:ch) : vprop
 
-val sent (#a_ch:G.erased Awc.ch) (c:ch) (eh:epoch_hash_entry a_ch) : prop
+val sent (#a_ch:G.erased Awc.ch) (c:ch) (eh:Formats.epoch_hash_entry) : prop
 
-val write (#a_ch:G.erased Awc.ch) (c:ch) (eh:epoch_hash_entry a_ch)
+val write (#a_ch:G.erased Awc.ch) (c:ch) (eh:Formats.epoch_hash_entry)
   : SteelT bool
       (writer c)
-      (fun b -> pure (b ==> sent c eh) `star` writer c)
+      (fun b -> pure (b ==> sent #a_ch c eh) `star` writer c)
 
 val read (#a_ch:G.erased Awc.ch) (c:ch)
-  : SteelT (epoch_hash_entry a_ch)
+  : SteelT Formats.epoch_hash_entry
       (reader c)
-      (fun eh -> pure (sent c eh) `star` reader c)
+      (fun eh -> pure (sent #a_ch c eh) `star` reader c)
